examples/low-level/huffman/huffman.fst
@@ -1,0 +1,114 @@
+(*--build-config
+    variables:LIB=../../../lib;
+    other-files:$LIB/ext.fst $LIB/set.fsi $LIB/set.fst $LIB/heap.fst $LIB/st.fst $LIB/all.fst $LIB/list.fst ../stack.fst ../listset.fst
+    $LIB/ghost.fst ../located.fst ../lref.fst ../stackAndHeap.fst ../sst.fst ../sstCombinators.fst $LIB/constr.fst ../word.fst $LIB/seq.fsi $LIB/seq.fst ../array.fsi
+     ../array.fst ../MD5Common.fst ../arrayAlgos.fst
+  --*)
+
+module Huffman
+
+open SST
+open SSTArray
+open ArrayAlgos
+
+open StackAndHeap
+open Stack
+
+open Lref
+
+assume val symbol_value_bound: nat
+
+type symbol_t = n:nat{n < symbol_value_bound}
+
+type node =
+  { frequency: lref int;
+    next: lref node;
+    zero_child: node;
+    one_child: node;
+    symbol: symbol_t;
+    code: lref string
+  }
+
+val live_node: n:node -> sm:smem -> GTot bool
+let live_node n sm =
+  liveRef n.frequency sm && liveRef n.next sm && liveRef n.code sm
+
+assume val null_node: unit -> PureMem node (fun sm0 -> True) (fun sm0 r -> b2t (live_node r sm0))
+
+val is_null: n:node -> PureMem bool (fun sm -> b2t (live_node n sm)) (fun sm r -> True)
+let is_null n = memread n.frequency = -1
+
+val g_is_null: n:node -> sm:smem{live_node n sm} -> GTot bool
+let g_is_null n sm = loopkupRef (n.frequency) sm = -1
+
+type node_list = lref node
+
+val live_node_list: l:node_list -> sm:smem{liveRef l sm} -> GTot bool
+let rec live_node_list l sm =
+  let n = loopkupRef l sm in
+  if not (live_node n sm) then false
+  else
+    if g_is_null n sm then true
+    else
+      live_node_list n.next sm
+
+val is_empty: l:node_list -> PureMem bool (fun sm0 -> )
+
+(*
+ * Nodes are not yet allocated on stack, would really like the located t and
+ * regionOf change (on-going discussion with Abhishek) before attempting that.
+ * When that happens, how do we write predicate on top most region before and after
+ * all refs point to same value after a pair is allocated on top most region ?
+ *)
+assume val mk_node: f:lref int -> n:lref node -> z:node -> o:node -> s:symbol_t -> c:lref string
+                    -> PureMem node
+                       (fun sm0 -> liveRef f sm0 /\ liveRef n sm0 /\ liveRef c sm0)
+                       (fun sm0 r -> live_node r sm0)
+
+type live_histogram (h:sstarray node) (sm:smem) =
+  liveArr sm h /\
+  (forall (i:nat). i < glength h sm ==> live_node (gindex h sm i) sm)
+
+(*
+ * Thus far only ensure that non empty regions in sm1, so that pop succeeds in caller
+ *)
+val compute_histogram: sstream: sstarray symbol_t -> histogram: sstarray node
+                       -> i:nat
+                       -> SST unit
+                          (fun sm0 -> isNonEmpty (st sm0)                                    /\
+                                      liveArr sm0 sstream /\ live_histogram histogram sm0    /\
+                                      glength histogram sm0 = symbol_value_bound             /\
+                                      i <= glength sstream sm0)
+                          (fun sm0 r sm1 -> b2t (isNonEmpty (st sm1)))
+let rec compute_histogram sstream histogram i =
+  if i = SSTArray.length sstream then ()
+  else
+    let sym = SSTArray.readIndex sstream i in
+    let the_leaf = SSTArray.readIndex histogram sym in
+    if is_null the_leaf then
+      let the_leaf' = mk_node (salloc 1) (salloc (null_node ())) (null_node ()) (null_node ()) sym (salloc "") in
+      SSTArray.writeIndex histogram sym the_leaf'
+    else
+      memwrite (the_leaf.frequency) ((memread the_leaf.frequency) + 1)
+
+val build_huffman_tree: histogram: sstarray node
+                        -> SST node
+                           (fun sm0 -> isNonEmpty (st sm0) /\ live_histogram histogram sm0)
+                           (fun sm0 r sm1 -> b2t (isNonEmpty (st sm1)))
+let build_huffman_tree histogram =
+  admit ()
+                                   
+
+val huffman_encode: sstream:sstarray symbol_t -> estream:sstarray byte
+                    -> SST (sstarray byte * nat * nat)
+                       (fun sm0 -> liveArr sm0 sstream /\ liveArr sm0 estream /\
+                                   glength sstream sm0 = glength estream sm0)
+                       (fun sm0 r sm1 -> True)
+let huffman_encode sstream estream =
+  pushStackFrame ();
+  let histogram = screate symbol_value_bound (null_node ()) in
+  compute_histogram sstream histogram 0;
+  let tree = build_huffman_tree histogram in
+  popStackFrame ();
+  admit ()
+  
